Proof almost complete

Dpda/CharPopStringPush.lean
@@ -84,16 +84,16 @@ structure CPSP_DPDA (Q S Γ) where
   F : Finset Q
   transition : CPSP_Transition Q S Γ
 
+def lift {α} (f : α → Option α) : Option α → Option α :=
+  fun u =>
+    match u with
+    | none => none
+    | some (a: α) => f a
+
 def CPSP_DPDA.run_n_steps {Q S Γ} [Fintype Q] [DecidableEq Q] [Fintype S /- Σ -/] [Fintype Γ]
   (M: CPSP_DPDA Q S Γ) (w: List S) (n: ℕ) : Option (CPSP_DPDA_IDesc Q S Γ) :=
   let step : CPSP_DPDA_IDesc Q S Γ -> Option (CPSP_DPDA_IDesc Q S Γ) := CPSP_Judge.stepTransition M.transition
-  Nat.repeat
-    (fun idesc =>
-      match idesc with
-      | none => none
-      | some idesc' => step idesc')
-    n
-    (some ⟨M.q0, w, []⟩)
+  Nat.repeat (lift step) n (some ⟨M.q0, w, []⟩)
 
 def CPSP_DPDA.membership_provable_in_n_steps {Q S Γ} [Fintype Q] [DecidableEq Q] [Fintype S /- Σ -/] [Fintype Γ]
   (M: CPSP_DPDA Q S Γ) (w: List S) (n: ℕ) : Bool :=
